src/triple/core.v
@@ -4,7 +4,7 @@
 Require Import Ssreflect.ssreflect Ssreflect.ssrfun Ssreflect.ssrbool Ssreflect.ssrnat Ssreflect.eqtype Ssreflect.tuple Ssreflect.seq Ssreflect.fintype.
 Require Import x86proved.bitsrep x86proved.bitsprops x86proved.bitsops x86proved.bitsopsprops x86proved.x86.procstate x86proved.x86.procstatemonad x86proved.pmapprops x86proved.x86.ioaction.
 Require Import x86proved.monad x86proved.monadinst x86proved.reader x86proved.spred x86proved.opred x86proved.spredtotal x86proved.septac x86proved.pointsto x86proved.pfun x86proved.cursor x86proved.writer.
-Require Import common_tactics.
+Require Import x86proved.common_tactics x86proved.common_definitions.
 
 Module Import tripleconfig.
   Export Ssreflect.ssreflect  Ssreflect.ssrfun Ssreflect.ssrbool (* for [==] notation *) Ssreflect.ssrnat (* for getting levels right *) Ssreflect.eqtype Ssreflect.tuple Ssreflect.seq (* for [++] *) Ssreflect.fintype.
@@ -21,15 +21,17 @@ Import Prenex Implicits.
 (** Hoare triple for machine state monad *)
 Definition TRIPLE (P:SPred) (c:ST unit) (O:OPred) (Q:SPred) :=
   forall s:ProcState, P s ->
-    exists f o, c s = (o, Success _ (f,tt)) /\ O (outputToActions o) /\ Q f.
+    exists f o, c s = (o, (f, Success _ tt)) /\ O (outputToActions o) /\ Q f.
 
 (** The general rule for dealing with [TRIPLE] by computation *)
 Lemma triple_fin (P:SPred) (c:ST unit) (O:OPred) (Q:SPred)
       (H : forall s:ProcState,
              P (toPState s)
              -> let outputs := fst (c s) in
-                match snd (c s) with
-                  | Success ftt =>  O (outputToActions outputs) /\ Q (toPState (fst ftt))
+                let f := fst (snd (c s)) in
+                let ex := snd (snd (c s)) in
+                match ex with
+                  | Success _ => O (outputToActions outputs) /\ Q (toPState f)
                   | Error _ => False
                 end)
 : TRIPLE P c O Q.
@@ -39,6 +41,7 @@ Proof.
   move => *.
   do ![ progress destruct_head False
       | progress destruct_head errorMT
+      | progress destruct_head OutputM
       | progress destruct_head Result
       | progress destruct_head prod
       | progress destruct_head unit
@@ -48,7 +51,7 @@ Qed.
 
 Lemma triple_simple_fin (P:SPred) outputs f (O:OPred) (Q:SPred)
       (H : forall s:ProcState, P (toPState s) -> O (outputToActions (outputs s)) /\ Q (toPState (f s)))
-: TRIPLE P (fun s => (outputs s, Success _ (f s, tt))) O Q.
+: TRIPLE P (fun s => (outputs s, (f s, Success _ tt))) O Q.
 Proof.
   apply triple_fin => s H' /=.
   by apply H.
@@ -62,12 +65,18 @@ Ltac triple_hnf :=
   let c' := hnf_under_binders c in
   change (TRIPLE P c' O Q).
 
+Ltac triple_post_compute :=
+  do ?[ progress ssr_autorewrite_with_matchdb
+      | progress autorewrite with matchdb
+      | progress unfold fst, snd
+      | progress cbv iota zeta ].
+
 Ltac triple_by_compute :=
   triple_hnf;
   apply triple_fin;
   let H := fresh "H" in
   let s := fresh "s" in
   (move => H s);
-    try (split; first by hnf; reflexivity);
-    cbv iota zeta;
-    simpl fst; simpl snd.
+    triple_post_compute;
+    repeat split;
+    triple_post_compute.
