src/common_definitions.v
@@ -1,4 +1,5 @@
 (** * Various useful general purpose notations and definitions *)
+Require Import Ssreflect.ssreflect.
 
 Notation eta_expand x := (fst x, snd x).
 
@@ -12,3 +13,176 @@ Fixpoint rep_apply n {A} (f : A -> A) (x : A) : A :=
     | 0 => x
     | S n' => f (rep_apply n' f x)
   end.
+
+  Lemma match_match_bool_option b T T' oT oF s n
+: match match b return option T with
+          | true => oT
+          | false => oF
+        end as o return T' o with
+    | Some x => s x
+    | None => n
+  end
+  = match b as b return T' (match b return option T with
+                              | true => oT
+                              | false => oF
+                            end) with
+      | true => match oT with
+                  | Some x => s x
+                  | None => n
+                end
+      | false => match oF with
+                   | Some x => s x
+                   | None => n
+                 end
+    end.
+Proof. destruct b, oT, oF; reflexivity. Defined.
+Lemma match_match_bool_pair b A B T xT xF P
+: match match b return prod A B with
+          | true => xT
+          | false => xF
+        end as p return T p with
+    | (x, y) => P x y
+  end
+  = match b as b return T (match b as b return prod A B with
+                             | true => xT
+                             | false => xF
+                           end) with
+      | true => match xT with
+                  | (x, y) => P x y
+                end
+      | false => match xF with
+                   | (x, y) => P x y
+                 end
+    end.
+Proof. destruct b, xT, xF; reflexivity. Defined.
+Lemma match_pair_eta A B (p : prod A B) T P
+: match p return T with
+    | (x, y) => P x y
+  end
+  = P (fst p) (snd p).
+Proof. destruct p; reflexivity. Defined.
+Lemma match_bool_fn b A B xT xF
+: match b as b return forall x : A, B b x with
+    | true => xT
+    | false => xF
+  end
+  = fun x : A => match b as b return B b x with
+                   | true => xT x
+                   | false => xF x
+                 end.
+Proof. destruct b; reflexivity. Defined.
+Lemma match_option_fn T (b : option T) A B s n
+: match b as b return forall x : A, B b x with
+    | Some k => s k
+    | None => n
+  end
+  = fun x : A => match b as b return B b x with
+                   | Some k => s k x
+                   | None => n x
+                 end.
+Proof. destruct b; reflexivity. Defined.
+Lemma match_option_match_pair_eta A B (p : option (prod A B)) T Ps Pn
+: match p return T with
+    | Some k => match k return T with
+                  | (x, y) => Ps x y
+                end
+    | None => Pn
+  end
+  = match p return T with
+      | Some k => Ps (fst k) (snd k)
+      | None => Pn
+    end.
+Proof. destruct p as [[? ?]|]; reflexivity. Defined.
+Lemma match_option_match_pair_eta_fun A B (p : option (prod A B)) T T' a Ps Pn
+: match p return T' with
+    | Some k => match k as k return T k -> T' with
+                  | (x, y) => Ps x y
+                end (a k)
+    | None => Pn
+  end
+  = match p return T' with
+      | Some k => Ps (fst k) (snd k) (a (fst k, snd k))
+      | None => Pn
+    end.
+Proof. destruct p as [[? ?]|]; reflexivity. Defined.
+Lemma match_option_comm_1 T (p : option T) A B (f : forall x : A, B x) s n
+: match p as p return B match p with
+                          | Some k => s k
+                          | None => n
+                        end with
+    | Some k => f (s k)
+    | None => f n
+  end
+  = f match p return A with
+        | Some k => s k
+        | None => n
+      end.
+Proof. destruct p; reflexivity. Defined.
+Lemma match_option_comm_2 T (p : option T) A B R (f : forall (x : A) (y : B x), R x y) (s1 : T -> A) (s2 : forall x : T, B (s1 x)) n1 n2
+: match p as p return R match p with
+                          | Some k => s1 k
+                          | None => n1
+                        end
+                        match p as p return B match p with Some k => s1 k | None => n1 end with
+                          | Some k => s2 k
+                          | None => n2
+                        end with
+    | Some k => f (s1 k) (s2 k)
+    | None => f n1 n2
+  end
+  = f match p return A with
+        | Some k => s1 k
+        | None => n1
+      end
+      match p as p return B match p with Some k => s1 k | None => n1 end with
+        | Some k => s2 k
+        | None => n2
+      end.
+Proof. destruct p; reflexivity. Defined.
+Definition match_option_comm_1_const T (p : option T) A B (f : A -> B) s n
+: (match p return B with
+     | Some k => f (s k)
+     | None => f n
+   end)
+  = (f match p return A with
+         | Some k => s k
+         | None => n
+       end)
+  := @match_option_comm_1 T p A _ f s n.
+Definition match_option_comm_2_const T (p : option T) A B R (f : A -> B -> R) s1 s2 n1 n2
+: (match p return R with
+     | Some k => f (s1 k) (s2 k)
+     | None => f n1 n2
+   end)
+  = (f match p return A with
+         | Some k => s1 k
+         | None => n1
+       end
+       match p return B with
+         | Some k => s2 k
+         | None => n2
+       end)
+  := @match_option_comm_2 T p A _ _ f s1 s2 n1 n2.
+Lemma match_bool_comm_1 (b : bool) A B (F : forall x : A, B x) t f
+: (if b as b return B (if b then t else f) then F t else F f)
+  = F (if b then t else f).
+Proof. destruct b; reflexivity. Defined.
+Lemma match_bool_comm_2 (b : bool) A B R (F : forall (x : A) (y : B x), R x y) t1 f1 t2 f2
+: (if b as b return R (if b then t1 else f1) (if b as b return B (if b then t1 else f1) then t2 else f2) then F t1 t2 else F f1 f2)
+  = F (if b then t1 else f1) (if b as b return B (if b then t1 else f1) then t2 else f2).
+Proof. destruct b; reflexivity. Defined.
+Definition match_bool_comm_1_const (b : bool) A R (F : A -> R) t f
+: (if b then F t else F f) = F (if b then t else f)
+  := @match_bool_comm_1 b _ _ F t f.
+Definition match_bool_comm_2_const (b : bool) A B R (F : A -> B -> R) t1 f1 t2 f2
+: (if b then F t1 t2 else F f1 f2) = F (if b then t1 else f1) (if b then t2 else f2)
+  := @match_bool_comm_2 b _ _ _ F t1 f1 t2 f2.
+Lemma match_bool_const (b : bool) A x : (if b return A then x else x) = x.
+Proof. destruct b; reflexivity. Defined.
+Lemma if_else_False_iff b P : (if b then P else False) <-> (P /\ (b = true)).
+Proof. destruct b; intuition. Qed.
+
+Hint Rewrite match_match_bool_option match_match_bool_pair match_pair_eta match_bool_fn match_option_fn match_option_match_pair_eta match_option_match_pair_eta_fun match_option_comm_1 match_option_comm_2 match_option_comm_1_const match_option_comm_2_const match_bool_comm_1 match_bool_comm_2 match_bool_comm_1_const match_bool_comm_2_const match_bool_const if_else_False_iff : matchdb.
+
+Ltac ssr_autorewrite_with_matchdb :=
+  do ?(progress rewrite ?match_match_bool_option ?match_match_bool_pair ?match_pair_eta ?match_bool_fn ?match_option_fn ?match_option_match_pair_eta ?match_option_match_pair_eta_fun ?match_option_comm_1 ?match_option_comm_2 ?match_option_comm_1_const ?match_option_comm_2_const ?match_bool_comm_1 ?match_bool_comm_2 ?match_bool_comm_1_const ?match_bool_comm_2_const ?match_bool_const ?if_else_False_iff).
