src/triple/morphisms.v
@@ -2,7 +2,7 @@
 Require Import x86proved.triple.core.
 Import triple.core.tripleconfig.
 
-Require Import Coq.Setoids.Setoid Coq.Program.Basics.
+Require Import Coq.Setoids.Setoid Coq.Program.Basics Coq.Classes.Morphisms.
 Require Import x86proved.common_tactics.
 
 Import Prenex Implicits.
@@ -12,6 +12,7 @@ Local Transparent ILFun_Ops ILPre_Ops.
 Local Ltac solve_morphism :=
   rewrite /TRIPLE; do ?[ split | move => ? ];
   do 6?[ by do !esplit; eauto with nocore
+       | by do !esplit; try hyp_rewrite <- *; eauto with nocore
        | progress destruct_head_hnf ex
        | progress destruct_head_hnf and
        | progress hnf in *; unfold lentails, ILFun_Ops, ILPre_Ops in *; hnf in *
@@ -30,4 +31,8 @@ Global Add Morphism (@TRIPLE) with signature lequiv ==> eq ==> lequiv ==> lequiv
 Proof. solve_morphism. Qed.
 
 Add Morphism (@TRIPLE) with signature lequiv ==> eq ==> eq ==> lequiv ==> iff as TRIPLE_mor4.
+Proof. solve_morphism. Qed.
+
+(** For dealing with programs *)
+Global Add Morphism (@TRIPLE) with signature eq --> (pointwise_relation ProcState eq) ==> eq ==> eq ==> impl as TRIPLE_morprogram.
 Proof. solve_morphism. Qed.
